theories/tree_valid_state.v
@@ -7,7 +7,7 @@ Section valid_tree.
   
   Fixpoint base_and s :=
     match s with
-    | And (CallS _ _ | CutS) r r1 => (r == r1) && base_and r1 (* should also say something about the program *)
+    | And (CallS _ _ | CutS) r r1 => (big_and r.1 r.2 == r1) && base_and r1 (* should also say something about the program *)
     | OK => true
     | _ => false
     end.
@@ -24,9 +24,10 @@ Section valid_tree.
     | t => base_and t
     end.
 
-  Fixpoint base_and_ko s :=
+  Definition base_and_ko s :=
     match s with
-    | And Bot r r1 => [&&base_and_ko r, (r == r1) & base_and_ko r1] (* should also say something about the program *)
+    | And Bot r r1 =>
+      [&& (big_and r.1 r.2 == r1) & base_and r1] (* should also say something about the program *)
     | Bot => true
     | _ => false
     end.
@@ -55,25 +56,22 @@ Section valid_tree.
       if is_dead A then valid_tree B
       else valid_tree A && (bbOr B)
     | And A B0 B => 
-      [&& valid_tree A,
+      valid_tree A &&
         if success A then valid_tree B 
-        else (B0 == B)
-        & (if success A || failed A then bbAnd B0 else base_and B0)]
+        else 
+          let B' := big_and B0.1 B0.2 in
+          B == B'
     end.
 
   Goal forall x r, (valid_tree (And CutS x r)) -> is_ko r = false.
-  Proof.
-    move=> x r/= /andP[] /eqP->.
-    elim: r => //-[]//.
-  Qed.
-
+  Proof. move=> x r/= /eqP->; rewrite is_ko_big_and//. Qed.
 
   Lemma is_dead_valid_tree {A} : is_dead A -> valid_tree A = false.
   Proof.
     elim: A => //.
       move=> A HA s B HB/=/andP[]dA dB.
       rewrite HA// dA HB//andbF//.
-    move=> A HA Bo ? B HB/=dA.
+    move=> A HA Bo B HB/=dA.
     rewrite HA// andbF//.
   Qed.
 
@@ -81,24 +79,16 @@ Section valid_tree.
   Proof. apply: contraPF => /is_dead_valid_tree->//. Qed.
 
   Lemma base_and_valid {A} : base_and A -> valid_tree A.
-  Proof.
-    elim A => //; clear => A HA B +; rewrite /base_or_aux //=; case: A HA => //=.
-      move=> p a _ + A + /andP [] /eqP H ; rewrite H; subst.
-      move=> _ H H1; rewrite H1//eqxx//.
-    move=> _ H _ _ /andP[/eqP<-] H1; rewrite H1//eqxx//.
-  Qed.
+  Proof. by elim: A => //=T _; case: T => //[p c|] [pr1 l] B HB /andP[/eqP<-]//=. Qed.
 
   Lemma valid_tree_big_and {pr l} : valid_tree (big_and pr l).
   Proof. apply: base_and_valid base_and_big_and. Qed.
 
+  Lemma base_and_ko_valid {B}: base_and_ko B -> valid_tree B.
+  Proof. elim: B => //; move=> []// HA B0 B HB/= /andP[/eqP<-]//. Qed.
+
   Lemma bbAnd_valid {A} : bbAnd A -> valid_tree A.
-  Proof.
-    move=>/orP[].
-      apply: base_and_valid.
-    elim: A=> //.
-    move=> []// _ B0 HB0 B HB/=/and3P[H/eqP->]bB.
-    rewrite eqxx /bbAnd bB orbT//base_and_ko_is_and//.
-  Qed.
+  Proof. by move=>/orP[/base_and_valid|/base_and_ko_valid]. Qed.
 
   Lemma big_or_aux_not_bot {pr l rs}: big_or_aux pr l rs != Bot.
   Proof. case: rs => [|[] xs]//=; case: l => //. Qed.
@@ -121,18 +111,20 @@ Section valid_tree.
     + move=> ??; case: F => // -[] //s1 r rs/=; rewrite bbOr_big_or_aux//. 
   Qed.
 
-  Lemma base_and_ko_valid {B}: base_and_ko B -> valid_tree B.
-  Proof.
-    elim: B => //.
-    move=> []// HA B0 _ B HB/= /and3P[bB0 /eqP <-] H.
-    by rewrite eqxx /bbAnd H orbT.
-  Qed.
-
   Lemma base_and_base_or_aux {A}: base_and A -> base_or_aux A.
   Proof. case: A => //. Qed.
 
   Lemma base_and_ko_base_or_aux_ko {A}: base_and_ko A -> base_or_aux_ko A.
   Proof. case: A => //. Qed.
+
+  Lemma base_and_failed {A}: base_and A -> failed A = false.
+  Proof. elim: A => //=-[]//=p a _ A HA B HB /andP[]//. Qed.
+
+  Lemma base_and_is_dead {A}: base_and A -> is_dead A = false.
+  Proof. move=>/base_and_failed; apply: contraFF is_dead_failed. Qed.
+
+  Lemma base_and_ko_is_ko {A}: base_and_ko A -> is_ko A.
+  Proof. elim: A => //=-[]//. Qed.
 
   Lemma bbOr_valid {B}:
     bbOr B -> valid_tree B.
@@ -140,38 +132,30 @@ Section valid_tree.
     move=> /orP [].
     elim B => //; clear.
     + move=> A HA s B HB/=/andP[bA bB].
-      rewrite HA ?base_and_base_or_aux// /bbOr bB HB// if_same//base_and_is_and//orbT//.
-    + move=> s; case: s => //[p t|] Ha B0 HB0 B HB /=/andP[/eqP->]bB; rewrite eqxx bB//.
+      by rewrite base_and_is_dead///bbOr bB HA//base_and_base_or_aux.
+    + by move=> s; case: s => //[p t|] Ha B0 B HB /=/andP[/eqP->]bB//.
     elim: B => //.
     + move=> A HA s B HB /= /andP [bA bB].
-      rewrite HB//HA?base_and_ko_base_or_aux_ko// /bbOr bB orbT if_same//base_and_ko_is_and//orbT//.
-    + move=> [] // HA B0 _ B HB /= /and3P[] bB0 /eqP <-.
-      rewrite /bbAnd bB0 eqxx // orbT//.
+      by rewrite HB//HA?base_and_ko_base_or_aux_ko// /bbOr bB orbT if_same.
+    + by move=> [] // HA B0 B HB /= /andP[]/eqP->; rewrite eqxx.
   Qed.
 
   Lemma base_and_base_and_ko_cut {B} : base_and B -> base_and_ko (cutr B).
-  Proof. 
-    elim: B => // A + B + C /=.
-    case: A => //=[_ _|] _ HB HC /andP [] /eqP <-bB; rewrite HB//eqxx//.
-  Qed.
+  Proof. by elim: B => //A; case: A => //. Qed.
 
   Lemma base_and_ko_base_and_ko_cutr {B} : base_and_ko B -> base_and_ko (cutr B).
-  Proof. 
-    elim: B => // -[]//_ A HA B HB/=/and3P[bA/eqP->bB].
-    rewrite HB//eqxx//.
-  Qed.
+  Proof. by elim: B => // -[]// _ l B HB /=/andP[/eqP<- H]; rewrite cutr2 eqxx//. Qed.
 
   Lemma base_and_base_and_ko_cutr {B} : base_and B -> base_and_ko (cutr B).
   Proof. 
-    elim: B => // A + B + C /=.
-    case: A => //=[_ _|] _ HB HC /andP [] /eqP <- hB; rewrite eqxx HB//.
+    by elim: B => // A; case: A => //[p c|] _ B0 B HB /=/andP[/eqP H1 H2]; rewrite HB// H1 eqxx.
   Qed.
   
   Lemma base_or_base_or_ko_cutr {B}: base_or_aux B -> base_or_aux_ko (cutr B).
   Proof.
     elim: B => //.
     + move=> A IHA s B IHB /= /andP [] /base_and_base_and_ko_cutr -> /IHB ->//.
-    + move=> a; case: a => //=[_ _|] _ B HB C HC /andP [] /eqP /[subst1] hC;
+    + move=> a; case: a => //=[_ _|] _ B C HC /andP [] /eqP /[subst1] hC;
       rewrite base_and_base_and_ko_cutr//eqxx//.
   Qed.
 
@@ -180,8 +164,7 @@ Section valid_tree.
     elim: B => //.
       move=> A HA s B HB /= /andP[bA bB].
       rewrite HB//base_and_ko_base_and_ko_cutr//.
-    move=> [] //= _ B0 _ B HB /and3P[] bB0 /eqP<- _.
-    rewrite base_and_ko_base_and_ko_cutr//eqxx//.
+    by move=> [] //= _ B0 B HB /andP[/eqP H1 H2]; rewrite base_and_ko_base_and_ko_cutr// -H1 cutr2 eqxx.
   Qed.
 
   (* Lemma valid_tree_compose_and {A2 B2 B02}: 
@@ -190,23 +173,22 @@ Section valid_tree.
         valid_tree B2.
   Proof. case: success => //; move=>/eqP->. apply: bbAnd_valid. Qed. *)
 
-  Lemma base_and_cutl {B0}:
+  (* Lemma base_and_cutl {B0}:
     base_and B0-> (B0 == OK) || base_and_ko (cutl B0).
   Proof.
-    elim: B0 => //= s; case: s => //= [_ _|] _ _ _ B HB /andP[/eqP->] bB;
+    elim: B0 => //= s; case: s => //= [_ _|] _ l B HB /andP[/eqP->] bB.
     rewrite eqxx !base_and_base_and_ko_cutr//.
-  Qed.
+  Qed. *)
 
-  Lemma base_ko_and_cutl {B0}:
+  (* Lemma base_ko_and_cutl {B0}:
     base_and_ko B0-> base_and_ko (cutl B0).
   Proof.
-    elim: B0; move=> //=[]//= _ _ _ B HB /and3P[_ /eqP->].
-    move=> /base_and_ko_base_and_ko_cutr->; rewrite eqxx//.
-  Qed.
+    by elim: B0; move=> //=[]//= _ l B HB /andP[/eqP H1 H2]; rewrite base_and_ko_base_and_ko_cutr// -H1 cutr2 eqxx.
+  Qed. *)
 
-  Lemma bbAnd_cutl{B0}:
+  (* Lemma bbAnd_cutl{B0}:
     bbAnd B0 -> (B0 == OK) || base_and_ko (cutl B0).
-  Proof. move=> /orP[/base_and_cutl|/base_ko_and_cutl]//->; rewrite orbT//. Qed.
+  Proof. move=> /orP[/base_and_cutl|/base_ko_and_cutl]//->; rewrite orbT//. Qed. *)
 
   Lemma bbOr_cutr {B}: bbOr B -> bbOr (cutr B).
   Proof.
@@ -221,17 +203,18 @@ Section valid_tree.
     move=> /base_and_ko_base_and_ko_cutr->; apply orbT.
   Qed.
 
-  Lemma valid_tree_cutr {A}: valid_tree A -> valid_tree (cutr A).
+  (* Lemma valid_tree_cutr {A}: valid_tree A -> valid_tree (cutr A).
   Proof.
     elim: A => //.
     - move=> A HA s B HB/=.
       rewrite is_dead_cutr.
       case: ifP => [dA vA|dA/andP[vA bB]]//; auto.
       rewrite bbOr_cutr//HA//.
-    - move=> A HA B0 HB0 B HB/=/and3P[vA].
-      case: ifP => /=[sA vB bB| sA /eqP -> bB].
-        rewrite HA//HB//bbAnd_cutr//success_cutr failed_cutr/=andbT.
-  Abort.
+    - move=> A HA B0 B HB/=/andP[vA].
+      case: ifP => /= [sA vB | sA ].
+        rewrite HA//HB// success_cutr//=failed_cutr.
+        (* rewrite HA//HB//bbAnd_cutr//success_cutr failed_cutr/=andbT. *)
+  Abort. *)
 
   Lemma valid_tree_cut {A}: success A -> valid_tree A -> valid_tree (cutl A).
   Proof.
@@ -240,8 +223,8 @@ Section valid_tree.
       case: ifP => //[dA sB vB| dA sA /andP[vA bB]]/=.
         rewrite dA HB//.
       rewrite is_dead_cutl dA HA// bbOr_cutr//.
-    move=> A HA B0 HB0 B HB /= /andP[sA sB] /and3P[vA].
-    rewrite sA/= => vB bB.
+    move=> A HA B0 B HB /= /andP[sA sB] /andP[vA].
+    rewrite sA/= => vB.
     rewrite success_cut sA HA//HB//=bbAnd_cutr//.
   Qed.
 
@@ -259,18 +242,15 @@ Section valid_tree.
         rewrite get_tree_Or/=dA IHB//.
       have /= := IHA s1 vA.
       case X: step => //= H; rewrite (step_not_dead _ dA X) H//bbOr_cutr//.
-    + move=> A HA B0 _ B HB s1 /=/and3P[vA].
-      case: ifP => [sA vB /= bB0 | sA /eqP->]/=.
+    + move=> A HA B0 B HB s1 /=/andP[vA].
+      case: ifP => [sA vB /= | sA]/=.
         rewrite succes_is_solved//=.
         have {HB} := HB (get_substS s1 A) vB.
         case X: step => //[C|C|C|C]/=vC; try by rewrite sA vA vC.
         rewrite success_cut sA/= vC valid_tree_cut//.
-        rewrite bbAnd_cutr//.
-      case: ifP => [fA bB|fA bB].
-        rewrite failed_expand//=vA sA eqxx bB/=fA//.
+      move=> /eqP -> {B HB}.
       have:= HA s1 vA.
-      case X: step => //[A'|A'|A'|A']/=vA'; last first;
-       [|rewrite //vA' base_and_valid///bbAnd bB eqxx !if_same//..].
+      case X: step => //[A'|A'|A'|A']/=vA'; only 1-3: by rewrite vA' valid_tree_big_and eqxx !if_same.
       have [? sA']:= expand_solved_same _ X; subst.
       congruence.
   Qed.
@@ -284,22 +264,13 @@ Section valid_tree.
   Qed.
 
   Lemma next_alt_aux_base_and {A}: base_and A -> next_alt false A = Some (A).
-  Proof. elim: A => //; move=>a; case: a => //=[p t|] _ B0 HB0 B HB s/andP[/eqP->bB]/=; rewrite HB//. Qed.
+  Proof. by elim: A => //[[]]//> _[]//. Qed.
 
   Lemma base_and_ko_failed {A}: base_and_ko A -> failed A.
   Proof. case: A => // -[]//. Qed.
 
   Lemma next_alt_aux_base_and_ko {A} b: base_and_ko A -> next_alt b A = None.
-  Proof. elim: A => //=; move=>/=[]//p a _ B0 HB0 B HB s/andP[/eqP->bB]/=. Qed.
-
-  Lemma base_and_failed {A}: base_and A -> failed A = false.
-  Proof. elim: A => //=-[]//=p a _ A HA B HB /andP[]//. Qed.
-
-  Lemma base_and_is_dead {A}: base_and A -> is_dead A = false.
-  Proof. move=>/base_and_failed; apply: contraFF is_dead_failed. Qed.
-
-  Lemma base_and_ko_is_ko {A}: base_and_ko A -> is_ko A.
-  Proof. elim: A => //=-[]//. Qed.
+  Proof. elim: A => //=[[]]//> _ []//. Qed.
 
   Lemma base_and_ko_is_dead {A}: base_and_ko A -> is_dead A = false.
   Proof. case: A => //-[]//. Qed.
@@ -336,7 +307,7 @@ Section valid_tree.
     elim: A b => //. 
     - move=> A HA s B HB /= b /andP[bA bB].
       rewrite !HB// next_alt_aux_base_and_ko// !if_same//.
-    - move=>/=[]//p a _ B0 HB0 B HB/andP[/eqP->bB]/=. 
+    - move=>/=[]//= _ []//=.
   Qed.
 
   Lemma next_alt_aux_base_or_none {A}: base_or_aux A -> next_alt false A = None -> A = Bot.
@@ -344,8 +315,7 @@ Section valid_tree.
     elim: A => //. 
     - move=> A HA s B HB /= /andP[bA bB].
       rewrite base_and_dead//next_alt_aux_base_and//.
-    - move=>A; case: A => //[p a|] _ B0 HB0 B HB/andP[/eqP->bB]/=;
-      rewrite next_alt_aux_base_and//. 
+    - move=>A; case: A => //[p a|] _ [pr l] B HB/= /andP[/eqP <- bB]//=.
   Qed.
 
   Lemma valid_tree_next_alt {A B b}: 
@@ -358,29 +328,22 @@ Section valid_tree.
     + move=> B _ _ [<-]//.
     + move=> A HA s B HB  C b/=.
       case: ifP => //[dA vB|dA /andP[vA bB]].
-        rewrite is_dead_next_alt//.
         case X: next_alt => //[D] [<-]/=.
         rewrite dA (HB _ _ vB X)//.
       case X: next_alt => [D|].
         move=>[<-]/=; rewrite bbOr_valid// bB (HA _ _ vA X) if_same//.
       case Y: next_alt => [D|]//[<-]/=; rewrite is_dead_dead (HB _ _ _ Y)//bbOr_valid//.
-    + move=> A HA B0 HB0 B HB  C b /=/and3P[vA].
-      case: ifP => /=[sA vB bB0|sA /eqP?]; subst.
-        rewrite success_failed//.
+    + move=> A HA [pr l] B HB  C b /= /andP[vA].
+      case: ifP => /=[sA vB|sA]; subst.
         case X: next_alt => [D|].
           move=>[<-]/=; rewrite vA sA/= (HB _ _ vB X)//.
         case Y: next_alt => //=[A'].
-        move: bB0 => /orPT[]/[dup]bB; last first.
-          move=> /(next_alt_aux_base_and_ko false) -> //.
-        move=> /next_alt_aux_base_and->[<-]/=.
-        by rewrite (base_and_valid bB) eqxx /bbAnd bB/= (HA _ _ vA Y) !if_same//.
-      case: ifP => fA bB; last first.
-        move=> [<-]/=; rewrite vA sA eqxx /bbAnd bB if_same//.
-      case X: next_alt => [D|]//.
-      move: bB => /orPT[]/[dup]bB; last first.
-        move=> /(next_alt_aux_base_and_ko false) -> //.
-      move=> /next_alt_aux_base_and->[<-]/=.
-      by rewrite (base_and_valid bB) eqxx /bbAnd bB/= (HA _ _ vA X) //!if_same//.
+        by move=> [<-]/=; rewrite (HA _ true)//= valid_tree_big_and eqxx !if_same.
+      move=> /eqP->{B HB}.
+      case: ifP => fA; last first.
+        by move=> [<-]/=; rewrite vA sA eqxx.
+      case X: next_alt => [D|]//=.
+      by move=> [<-]/=; rewrite (HA _ false)//= eqxx valid_tree_big_and !if_same.
     Qed.
 
   Lemma valid_tree_run {s1 A s2 B b}:
@@ -402,4 +365,8 @@ Section valid_tree.
 
   Lemma base_and_ko_succes {B}: base_and_ko B -> success B = false.
   Proof. elim: B => // -[]//=. Qed.
+
+  Lemma base_or_aux_is_ko {A}: base_or_aux A -> is_ko A = false.
+  Proof. move=> /base_or_failed/failed_is_ko//. Qed.
+
 End valid_tree.
