theories/t2l_prop.v
@@ -104,7 +104,7 @@ Section NurProp.
     Proof.
       elim: A l s => //.
       - move=> A HA s B HB/= l s1/andP[dA dB]; rewrite HB// HA//.
-      - move=> A HA B0 HB0 B HB l s1 /=dA; rewrite HA//=.
+      - move=> A HA B0 B HB l s1 /=dA; rewrite HA//=.
     Qed.
 
     Lemma t2l_dead {A l s}: is_dead A -> t2l A s l = nilC.
@@ -124,10 +124,19 @@ Section NurProp.
     Proof.
       elim: A => //=.
       - by eexists.
-      - move=> s; case: s => //=[p a|] _ B0 _ B HB/andP[/eqP->bB]; have [hd H]/= := HB bB.
+      - move=> s; case: s => //=[p a|] _ B0 B HB/andP[/eqP ? bB]; subst; have [hd H]/= := HB bB.
           by eexists => l s/=; rewrite H//= !cat0s?H//.
         eexists => l s/=; rewrite H//= !cat0s?H//.
         rewrite sub0n drop0// H//.
+    Qed.
+
+    Lemma s2l_big_and p1 r1 s l: 
+      t2l (big_and p1 r1) s l = (s, a2gs p1 r1) ::: nilC.
+    Proof. 
+      elim: r1 => //=-[|t] xs H//=; rewrite H/=.
+      - rewrite drop0 take0 make_lB0_empty1 !cat0s cats0.
+        rewrite/make_lB01/=map_cons cat_cons cat0s//.
+      - rewrite make_lB0_empty1 cats0/make_lB01/= map_cons cat_cons cat0s//.
     Qed.
 
     Lemma base_and_empty_ca {A B}:
@@ -135,7 +144,7 @@ Section NurProp.
     Proof.
       elim: A B => //=.
         move=> B _ /(_ nilC empty) [<-]//.
-      move=> a; case: a => //=[p a|] _ _ _ B HB /=C /andP[/eqP->bB].
+      move=> a; case: a => //=[p a|] _ B0 B HB /=C /andP[? bB]; subst.
         have [hd H]:= base_and_t2l bB.
         move: HB => /(_ _ bB) -/(_ _ H) H1 /(_ nilC empty).
         rewrite H//=/empty_caG => -[?]; subst; rewrite/empty_caG all_cat//.
@@ -175,7 +184,7 @@ Section NurProp.
       have [hd H]:= base_and_t2l H1.
       rewrite H all_cons.
       rewrite (base_and_empty_ca H1 H)//.
-    - move=> A; case: A => //=[p a|] _ _ _ B HB s1 /andP[/eqP->]bB.
+    - move=> A; case: A => //=[p a|] _ B0 B HB s1 /andP[/eqP? bB]; subst.
         have [hd H]:= base_and_t2l bB.
         rewrite H/=/all//=/empty_caG/all/=.
         have:= (base_and_empty_ca bB H); rewrite /empty_caG/all/= => H1; rewrite H1//.
@@ -201,7 +210,7 @@ Section NurProp.
     - move=> B bt _ [<-]//.
     - move=> A HA s' B HB C bt /andP[H1 H2].
       rewrite base_and_dead// next_alt_aux_base_and// => -[<-]//=.
-    - move=> A; case: A => //=[p c|] _ _ _ B HB C bt /andP[/eqP-> bB][<-]//.
+    - move=> A; case: A => //=[p c|] _ [p1 l] B HB C bt /andP[/eqP? bB][<-]; subst => //.
   Qed.
 
   Lemma success_t2l {A s m} s1:
@@ -212,7 +221,7 @@ Section NurProp.
     elim: A m s s1 => //.
     - move=> A HA sb B HB/= m s s1.
       case: ifP => [dA vB sB|dA /andP[vA bB] sA].
-        rewrite is_dead_next_alt// /=!(t2l_dead dA)!cat0s.
+        rewrite /=!(t2l_dead dA)!cat0s.
         have H := [elaborate HB nilC sb sb vB sB].
         rewrite H//=.
         case X: next_alt => //[B'|]/=.
@@ -229,31 +238,17 @@ Section NurProp.
         rewrite (t2l_dead is_dead_dead)// (base_or_aux_next_alt_t2l bB X)//.
       have -> /=:= next_alt_aux_base_or_none bB X.
       by rewrite (t2l_dead is_dead_dead)/=.
-    - move=> A HA B0 HB0 B HB m s1 s2 /= /and3P[vA] + + /andP[sA sB].
-      rewrite sA/==> vB bB.
-      have {}HA := HA _ _ _ vA sA. repeat erewrite HA => /=.
+    - move=> A HA [p l] B HB m s1 s2 /= /andP[vA +] /andP[sA sB].
+      rewrite sA/= => vB.
+      have {}HA := HA _ _ _ vA sA; repeat erewrite HA => /=.
       have {}HB := HB _ _ _ vB sB; repeat erewrite HB => /=.
-      rewrite success_failed//.
-      have:= bB; rewrite/bbAnd=>/orP[]{}bB; last first.
-        rewrite !(base_and_ko_t2l bB)//=.
-        rewrite (next_alt_aux_base_and_ko _ bB).
-        case X: next_alt => //=[B'|].
-          rewrite (HA _ _ s2)/=.
-          rewrite (base_and_ko_t2l bB)//=.
-        rewrite !(t2l_dead is_dead_dead)/=.
-        case: next_alt; rewrite !(t2l_dead is_dead_dead)//=.
-      have [hd H3] := base_and_t2l bB.
-      rewrite !H3/=!make_lB01_empty2.
-      erewrite HB => //=; rewrite cat_cons; f_equal.
       case X: (next_alt _ B) => [B'|]/=.
-        rewrite (HA _ _ s2) //= H3 /=.
-        f_equal.
-        rewrite make_lB01_empty2//.
+        by rewrite (HA _ _ s2) //= H3 /=.
       rewrite !(t2l_dead is_dead_dead)/=.
       case W: next_alt => //=[A'|].
-        rewrite next_alt_aux_base_and//=.
-        case Z: t2l => //= [[sx x]xs]/=.
-        rewrite H3//=H3//.
+        rewrite make_lB01_empty2 cat_cons cat0s; f_equal.
+        case: t2l => //= -[s b] a.
+        rewrite s2l_big_and//.
       by rewrite !(t2l_dead is_dead_dead)/=.
   Qed.
 
@@ -267,14 +262,10 @@ Section NurProp.
       elim: A s1 l1 s2 l2 => //=.
       - move=> A HA s B HB s1 l1 s2 l2; rewrite !size_add_ca_deep!size_cat.
         by f_equal; auto.
-      - move=> A HA B0 HB0 B HB /=s1 l1 s2 l2.
+      - move=> A HA B0 B HB /=s1 l1 s2 l2.
         have:= HA s1 l1 s2 l2.
         do 2 case: (t2l A) => //=.
         move=> [s x] xs [s3 y] ys; rewrite !size_cons => -[]H.
-        have:= HB0 s1 l1 s2 l2.
-        do 2 case: (t2l B0) => //=.
-          rewrite !size_map//.
-        move=> [s5 w] [|??] [s6 z] [|??]//= _.
         set X:= make_lB0 _ _.
         set Y:= make_lB0 _ _.
         rewrite !size_cat !size_map !size_add_deep H; f_equal.
@@ -312,34 +303,20 @@ Section NurProp.
       have [s2 [x[xs H]]] := HA vA fA s1 X.
       have [s3 [y[ys ->]]]:= s2l_cons H s1 X.
       by do 3 eexists.
-    - move=> A HA B0 _ B HB/= /and3P[vA]+++s1 l/=.
-      case: ifP => /=[sA vB bB0|sA /eqP->]/=.
+    - move=> A HA B0 B HB/= /andP[vA] ++ s1 l.
+      case: ifP => /=[sA vB|sA]/=.
         rewrite success_failed//==>fB.
+        rewrite/t2l_cons/=.
         have X := success_t2l empty vA sA.
         rewrite X/=.
         have [s2 [x[xs {}HB]]]:= HB vB fB s1 l.
-        move: bB0.
-        rewrite /bbAnd => //.
-        case bB: base_and; last first => /=.
-          move=> {}bB.
-          rewrite (base_and_ko_t2l bB)/=.
-          have [s[hd [tl ->]]]:= s2l_cons HB (get_substS s1 A) l.
-          by do 3 eexists.
-        move=> _.
-        have [hd H1]:= base_and_t2l bB.
-        rewrite H1/=.
         set Y:= make_lB0 _ _.
         have [s[hd1 [tl ->]]]:= s2l_cons HB (get_substS s1 A) (Y++l).
         by do 3 eexists.
-      rewrite orbF => + fA; rewrite fA => bB.
-      have [s2 [x[xs ->]]]:= HA vA fA s1 l.
-      have fB:= base_and_failed bB.
-      have [hd H]:= base_and_t2l bB.
-      rewrite H/=.
-      set X:= make_lB0 _ _.
-      have[s3 [y[ys{}HB]]]:= HB (base_and_valid bB) fB s1 (X ++ l).
-      have [s[hd1 [tl ->]]]:= s2l_cons HB s2 (X++l).
-      by do 3 eexists.
+      move=> /eqP ->{B HB}; rewrite orbF => fA.
+      have [s2 [x[xs ->]]]:= HA vA fA s1 l => /=.
+      rewrite s2l_big_and cat_cons.
+      by repeat eexists.
   Qed.
 
   Lemma expand_t2l_cons {s A r}:
@@ -354,7 +331,7 @@ Section NurProp.
       move=>/orP[]/andP[bA bB].
         rewrite base_and_dead// next_alt_aux_base_and//.
       rewrite base_and_ko_t2l// base_or_aux_ko_t2l//.
-    - move=> A; case: A => //=[p a|] _ B0 _ B HB s s1 l/=; rewrite /bbOr/=orbF => /andP[/eqP->bB].
+    - move=> A; case: A => //=[p a|] _ [p' l'] B HB s s1 l//=.
   Qed.
 
   Lemma expand_failure_next_alt_none_empty {A s1 s3 E l b}:
@@ -367,7 +344,7 @@ Section NurProp.
     - move=> A HA s B HB/=s1 s2 E l b.
       case: ifP => //[dA vB|dA/andP[vA bB]].
         case eB: step => //[B'][<-]/=.
-        rewrite is_dead_next_alt// dA.
+        rewrite dA//=.
         case nB': next_alt => [[]|]// _.
         by rewrite (HB _ _ _ _ _ vB eB nB')/=t2l_dead//.
       case eA: step => //[A'][<-]/=.
@@ -379,32 +356,22 @@ Section NurProp.
       move: bB; rewrite /bbOr => /orP[]; last first.
         move=> /base_or_aux_ko_t2l->//.
       move=> H; rewrite (next_alt_aux_base_or_none H nB')//.
-    - move=> A HA B0 _ B HB s2 s3 C l b/=/and3P[vA].
+    - move=> A HA [p l'] B HB s2 s3 C l b/=/andP[vA].
       case eA: step => //[A'|A'].
         have [? fA]:= expand_failed_same _ eA; subst.
-        rewrite (failed_success _ fA) fA/==>/eqP->bB[<-]/=.
-        rewrite fA.
-        case nA: next_alt => [D|].
-          move: bB; rewrite/bbAnd=>/orP[]bB//; last first.
-            rewrite (base_and_ko_t2l bB)//=.
-            case: t2l => // [[??]?].
-            by rewrite (base_and_ko_t2l bB)//=.
-          by rewrite next_alt_aux_base_and//.
+        rewrite failed_success// => /eqP ->[<-]/=.
+        rewrite fA failed_success//.
+        case nA: next_alt => [D|]//= _.
         by rewrite (HA _ _ _ _ _ vA eA nA)//.
       have [? sA]:= expand_solved_same _ eA; subst.
-      rewrite sA => vB bB0.
+      rewrite sA => vB.
       case eB: step => //[B'][<-]/=.
       rewrite success_failed//sA.
       case nB': next_alt => [[]|]//.
       rewrite (success_t2l empty) => //=.
-      move /orP: bB0 => []bB; last first.
-        rewrite base_and_ko_t2l//=.
-        rewrite (HB _ _ _ _ _ vB eB nB')//.
-      have [hd H]:= base_and_t2l bB.
-      rewrite H/= (HB _ _ _ _ _ vB eB nB')// make_lB01_empty1.
-      rewrite (next_alt_aux_base_and bB)//.
-      case X: next_alt => //.
-      by rewrite/= !(t2l_dead is_dead_dead)/=.
+      case X: next_alt => //= _.
+      rewrite/= !(t2l_dead is_dead_dead)/=.
+      by rewrite (HB _ _ _ _ _ vB eB nB')//.
   Qed.
 
 
@@ -421,17 +388,14 @@ Section NurProp.
         rewrite 2!(t2l_dead dA) (HB _ _ _ _ eB)//dA//.
       case eA: step => //[A'][<-]/=.
       have ->// := HA _ _ _ _ eA.
-    - move=> A HA B0 _ B HB s sx C l/=.
+    - move=> A HA B0 B HB s sx C l/=.
       case eA: step => //[A'|A'].
         have [? H] := expand_failed_same _ eA; subst.
         move=> [<-]//=.
       have [? sA] := (expand_solved_same _ eA); subst.
       case eB: step => //[B'][<-]/=.
       case: t2l => //= -[s2 x] xs.
-      case: t2l => //=.
-        rewrite (HB _ _ _ _ eB)//.
-      move=> [s3 y] []//; f_equal.
-      rewrite (HB _ _ _ _ eB)//.
+      by rewrite (HB _ _ _ _ eB).
   Qed.
 
   Lemma base_or_aux_next_alt_some {B s2 D l}:
@@ -444,7 +408,7 @@ Section NurProp.
       rewrite base_and_dead//.
       rewrite (next_alt_aux_base_and bA)//.
       move=>[<-]//=; subst; rewrite base_and_dead//.
-    - move=> A; case: A => //[p a|] _ B0 _ B HB s2 C l/=/andP[/eqP->bB][<-]//.
+    - move=> A; case: A => //[p a|] _ [p' l'] B HB s2 C l/=/andP[? bB][<-]//.
   Qed.
 
   Lemma add_ca_deep_map_empty ca X:
@@ -471,15 +435,6 @@ Section NurProp.
     rewrite/empty_ca.
     elim: rs => //=-[s b l]/= H.
     rewrite all_cons empty_ca_atoms//.
-  Qed.
-
-  Lemma s2l_big_and p1 r1 s l: 
-    t2l (big_and p1 r1) s l = (s, a2gs p1 r1) ::: nilC.
-  Proof. 
-    elim: r1 => //=-[|t] xs H//=; rewrite H/=.
-    - rewrite drop0 take0 make_lB0_empty1 !cat0s cats0.
-      rewrite/make_lB01/=map_cons cat_cons cat0s//.
-    - rewrite make_lB0_empty1 cats0/make_lB01/= map_cons cat_cons cat0s//.
   Qed.
 
   Lemma s2l_big_or k s {p1 b bs ca gs}:
@@ -511,35 +466,34 @@ Section NurProp.
     elim: A s b => //.
     - move=> A HA s B HB s2 b/=.
       case: ifP => [dA vB fB|dA /andP[vA bB] fA].
-        rewrite is_dead_next_alt//.
         case X: next_alt => [C|]//.
         move=> _ l; rewrite (HB _ _ _ _ X)// t2l_dead//.
       case Y: next_alt => [[]|]//.
       case Z: next_alt => [D|]// _ l.
       rewrite (HA s2 b)//=.
       rewrite (bbOr_next_alt_none bB Z)//.
-    - move=> A HA B0 HB0 B HB s2 b/=/and3P[vA]++++l.
-      case: ifP => /=[sA vB bB0|sA/eqP->].
+    - move=> A HA [p' l'] B HB s2 b/=/andP[vA]+++l.
+      case: ifP => /=[sA vB|sA].
         rewrite (success_t2l empty)//=.
         rewrite success_failed//= => fB.
         case X: next_alt => [[]|]//.
-        move/orP: bB0 => []bB; last first.
-          by rewrite base_and_ko_t2l//= (HB _ _ _ _ X)//.
-        have [hd H]:= base_and_t2l bB.
-        rewrite H/=(HB _ _ _ _ X)//.
+        rewrite /=(HB _ _ _ _ X)//.
         case W: next_alt => //=.
-        rewrite next_alt_aux_base_and//.
         by rewrite !(t2l_dead is_dead_dead)/=.
       rewrite orbF => +fA; rewrite fA.
-      move => bB.
-      case X: next_alt => //[A'|].
-        move/orP: bB => []bB; last first.
-          rewrite (base_and_ko_t2l bB)/=.
-          rewrite next_alt_aux_base_and_ko// => _.
-          case W: t2l => //[[??]?].
-          rewrite base_and_ko_t2l//.
-        rewrite next_alt_aux_base_and//.
-      rewrite (HA _ _ vA fA X)//.
+      move=> H.
+      case X: next_alt => //= _.
+      by rewrite (HA _ _ vA fA X)//.
+  Qed.
+
+  Lemma t2l_cutr_empty {A s l}:
+    valid_tree A -> t2l (cutr A) s l = nilC.
+  Proof.
+    elim: A s l => //.
+    - move=> A HA s B HB s1 l /=; case: ifP => //[dA vB|dA /andP[vA bB]].
+        rewrite HB//t2l_dead//is_dead_cutr//.
+      rewrite HA//HB//bbOr_valid//.
+    - move=> A HA B0 B HB s l /=/andP[oA vA]; rewrite HA//.
   Qed.
 
   Lemma failed_next_alt_some_t2l {A B l b} s3:
@@ -549,7 +503,6 @@ Section NurProp.
     elim: A s3 B l b => //.
     - move=> A HA s B HB s3 C l b/=.
       case: ifP => [dA vB fB|dA /andP[vA bB] fA].
-        rewrite is_dead_next_alt//.
         case X: next_alt => [D|]//[<-]/=.
         by rewrite !(t2l_dead dA)//=(HB _ _ _ _ vB fB X)//.
       case X: next_alt => [A'|]//.
@@ -560,43 +513,24 @@ Section NurProp.
       case Y: next_alt => [A'|]//[<-]/=.
       rewrite (base_or_aux_next_alt_some bB Y) !add_ca_deep_cat (failed_next_alt_none_t2l vA fA X).
       rewrite (t2l_dead is_dead_dead)//.
-    - move=> A HA B0 HB0 B HB s1 C l b /=/and3P[vA].
-      case: ifP => /=[sA vB bB0|sA/eqP->].
+    - move=> A HA [p' l'] B HB s1 C l b /=/andP[vA].
+      case: ifP => /=[sA vB |sA ].
         rewrite success_failed//= => fB.
         case X: next_alt => [D|]//.
           move=>[?]/=; subst => /=.
           have{}HB := (HB _ _ _ _ vB fB X).
           case Z: t2l => //[[s4 g]gs].
           rewrite HB.
-          case W: t2l => //[[s5 g1][]]//=.
-          by rewrite HB//.
-        case Y: next_alt => //[A'].
-        move/orP:bB0 => []bB; last first.
-          rewrite next_alt_aux_base_and_ko//.
-        have [hd H]:= base_and_t2l bB.
-        rewrite next_alt_aux_base_and// => -[<-]/=.
-        rewrite (success_t2l s1)//=H/=.
+          by case W: t2l => //[[s5 g1][]]//=.
+        case Y: next_alt => //=[A'][<-]{C}.
+        rewrite (success_t2l s1)//=.
         rewrite (failed_next_alt_none_t2l _ _ X)//Y.
         case: t2l => //[[s2 x]xs].
-        by rewrite H//.
-      rewrite orbF => + fA.
-      rewrite fA => bB.
-      case X: next_alt => //=[A'].
-      move/orP:bB => []bB; last first.
-        rewrite next_alt_aux_base_and_ko//.
-      have [hd H]:= base_and_t2l bB.
-      rewrite next_alt_aux_base_and// => -[<-]/=.
-      by rewrite (HA _ _ _ _ vA fA X)//.
-  Qed.
-
-  Lemma t2l_cutr_empty {A s l}:
-    valid_tree A -> t2l (cutr A) s l = nilC.
-  Proof.
-    elim: A s l => //.
-    - move=> A HA s B HB s1 l /=; case: ifP => //[dA vB|dA /andP[vA bB]].
-        rewrite HB//t2l_dead//is_dead_cutr//.
-      rewrite HA//HB//bbOr_valid//.
-    - move=> A HA B0 _ B HB s l /=/and3P[oA vA]; rewrite HA//.
+        by rewrite s2l_big_and//.
+      rewrite orbF => /eqP->{B HB} fA.
+      rewrite fA.
+      case X: next_alt => //=[A'][<-]{C}.
+      by rewrite (HA _ _ _ _ vA fA X)//=.
   Qed.
 
 
@@ -634,6 +568,10 @@ Section NurProp.
     base_and A -> get_substS s1 A = s1.
   Proof. elim: A s1 => //=-[]//= _ _ _ B0 _ B HB s1 /andP[H1]; apply: HB. Qed.
 
+  Lemma get_substS_big_and A pr s1:
+    get_substS s1 (big_and pr A) = s1.
+  Proof. apply/get_substS_base_and/base_and_big_and. Qed.
+
 
   Lemma expand_cb_same_subst1 {A B s1}:
   (* TODO: put this prop inside s2l_CutBrothers *)
@@ -642,13 +580,13 @@ Section NurProp.
     elim: A B s1 => //=.
     - move=> B s1 _ [<-]//.
     - move=> A HA s B HB C s1;  case: ifP => dA; case: step => //.
-    - move=> A HA B0 _ B HB C s1 /and3P[vA].
+    - move=> A HA B0 B HB C s1 /andP[vA].
       case e: step => //[A'|A'].
-        rewrite (step_not_solved _ e)//=(step_not_failed _ e)//=.
-        move=>/eqP-> bB [<-]/=; rewrite (get_substS_base_and bB)// if_same.
+        rewrite (step_not_solved _ e)//=.
+        move=> /eqP->[<-]/=; rewrite get_substS_big_and if_same.
         rewrite !(HA _ _ vA e)//.
       have [? sA] := expand_solved_same _ e; subst.
-      rewrite sA/= => vB bB.
+      rewrite sA/= => vB.
       case e1: step => //=[B'][<-]/=; rewrite success_cut sA ges_subst_cutl//.
       rewrite !(HB _ _ vB e1)//.
   Qed.
@@ -660,13 +598,10 @@ Section NurProp.
     - move=> A HA s B HB s1 l /=; case: ifP => [dA vB sB | dA /andP[vA bB] sA]/=.
         rewrite HB// t2l_dead//=.
       by rewrite (t2l_cutr_empty (bbOr_valid bB))/=cats0 HA.
-    - move=> A HA B0 _ B HB s l/=/and3P[vA] + +/andP[sA sB].
-      rewrite sA/==> vB bB0.
-      rewrite HA//.
-      rewrite /= is_ko_t2l//=?is_ko_cutr//.
-      rewrite make_lB01_empty2.
-      rewrite (success_t2l empty)/=?success_cut// ?valid_tree_cut// ges_subst_cutl//.
-      f_equal; rewrite next_alt_cutl//=t2l_dead//is_dead_dead//.
+    - move=> A HA B0 B HB s l/=/andP[vA] +/andP[sA sB].
+      rewrite sA/= => vB.
+      rewrite HA//= make_lB01_empty2 make_lB0_empty1 cats0 cat0s.
+      by rewrite HB//.
   Qed.
 
 
@@ -682,43 +617,29 @@ Section NurProp.
     - move=> //=?????[<-]/=; by do 2 eexists.
     - move=> A HA s B HB sA s1 C l1 /=.
       by case: ifP => [dA vB|dA/andP[vA bB]]; case eB: step => //[s1' B'][??]; subst.
-    - move=> A HA B0 _ B HB sA s1 C l1/=/and3P[vA].
+    - move=> A HA B0 B HB sA s1 C l1/=/andP[vA].
       case eA: step => //[A'|A'].
-        rewrite (step_not_solved _ eA notF)/=(step_not_failed _ eA notF).
-        move=>/eqP->bB [<-]/=.
-        have [y  H1] /=:= base_and_t2l bB.
+        rewrite (step_not_solved _ eA notF)/=.
+        move=>/eqP-> [<-]/={B HB}.
         have {HA}[x [tl [H3 [H4 H5]]]] := HA sA _ _ l1 vA eA.
-        have /= H6 := base_and_empty_ca bB H1.
         do 2 eexists; repeat split.
-        - rewrite H1 H3/= take0 drop0 make_lB0_empty1 H1 !cat_cons//(get_substS_base_and bB)//.
-        - move=> l sB; rewrite H1/= H4/=H1 cats0 empty_caG_add_deepG//empty_caG_add_deepG//.
-          rewrite (get_substS_base_and bB)// if_same//.
+        - rewrite H3/= s2l_big_and/= take0 drop0 make_lB0_empty1//.
+        - move=> l sB; rewrite H4/= s2l_big_and cats0 empty_caG_add_deepG//empty_caG_add_deepG//.
+          rewrite get_substS_big_and if_same//.
         - rewrite !empty_caG_add_deepG///empty_caG all_cat.
-          apply/andP; split => //; apply:H6.
+          apply/andP; split => //; apply: empty_ca_atoms.
       have [? sAx] := expand_solved_same _ eA; subst.
-      rewrite sAx/==> vB bB0.
+      rewrite sAx/==> vB.
       case eB: step => //[B'] [<-]/=.
       rewrite (success_t2l empty (valid_tree_expand _ vA eA) sAx)/=.
-      have [H2|[hd[H2 H3]]] := bbAnd_t2l bB0; rewrite H2/=.
-        have {HB}[x[tl [H H1]]] := HB (get_substS sA A')  _ _ l1 vB eB.
-        do 2 eexists; repeat split; try eassumption.
-        rewrite H/make_lB01 map_cons; f_equal; f_equal; repeat split => //.
-        move=> l sb.
-        rewrite t2l_cutl//=.
-        have vB0 := bbAnd_valid bB0.
-        rewrite t2l_cutr_empty//=.
-        rewrite H1 success_cut sAx make_lB01_empty2 ges_subst_cutl//.
-        rewrite H1//.
       set X:= make_lB0 _ _.
       have [x[tl [H [H1 H4]]]] := HB (get_substS sA A') _ _ (X++l1) vB eB.
       rewrite H//=.
       do 2 eexists; split; try eassumption.
-      rewrite make_lB01_empty2//=cat_cons; f_equal; f_equal; split => //.
+      by rewrite make_lB01_empty2//=.
       rewrite H4; split => //.
       move=> //l sB.
-      have vB0 := bbAnd_valid bB0.
       rewrite t2l_cutl//=.
-      rewrite t2l_cutr_empty//=.
       rewrite success_cut sAx ges_subst_cutl//H1//.
   Qed.
 
@@ -736,26 +657,19 @@ Section NurProp.
       have [sy[y[ys H]]] := failed_t2l vA fA s1 SB.
       rewrite H; case: y H => //= H [??]; subst.
       by apply: HA H.
-    - move => A HA B0 _ B HB s bt s1 xs /and3P[vA].
+    - move => A HA B0 B HB s bt s1 xs /andP[vA].
       case fA: failed => //=.
-      case: ifP => //=[sA vB bB sB fB|sA /eqP->{B0} bB _I _I1].
+      case: ifP => //=[sA vB sB fB|sA /eqP->{B HB} _I _I1].
         rewrite (success_t2l empty) => //=.
-        move/orPT: bB => []bB; last first.
-          rewrite base_and_ko_t2l//= make_lB01_empty2 => H.
-          by apply: HB H.
-        have [h H]:= base_and_t2l bB.
-        rewrite H/= make_lB01_empty2/=.
         set ml := make_lB0 _ _.
         have [s2'[y[ys H1]]] := [elaborate failed_t2l vB fB (get_substS s A) (ml ++ bt)].
         rewrite H1/=.
         case: y H1 => //= H1 [??]; subst.
         by apply: HB H1.
       have [s2'[y[ys H]]] := failed_t2l vA fA s bt.
-      have [hd H1]:= base_and_t2l bB.
-      have E := base_and_empty_ca bB H1.
-      rewrite H/=H1/=!H1/= => -[?+?]; subst.
-      case: y H; rewrite//=cat0s => H?; subst.
-      by apply: HA H.
+      rewrite H/= s2l_big_and cat_cons cat0s => -[?+?]; subst.
+      case: y H; rewrite//= cat0s => H1 H2.
+      by apply/HA/H1.
   Qed.
 
   Lemma expand_cb_failedF {s1 A B}:
@@ -766,15 +680,14 @@ Section NurProp.
     - move=> B _ _ [<-]//.
     - move=> A HA s B HB C s1.
       case: ifP => //[dA fB|dA fA]; case e: step => //.
-    - move=> A HA B0 _ B HB C s1 /and3P[vA].
+    - move=> A HA B0 B HB C s1 /andP[vA].
       case e: step => //[A'|A'].
-        rewrite (step_not_solved _ e)//(step_not_failed _ e)//=.
-        move=>/eqP->bB [<-]/=.
-        rewrite (base_and_failed bB) andbF.
-        rewrite (HA _ _ vA e)//(step_not_failed e)//.
+        rewrite (step_not_solved _ e)//.
+        move=>/eqP->{B HB} [<-]/=.
+        by rewrite (HA _ _ vA e)//= failed_big_and andbF.
       have [? sA] := expand_solved_same _ e; subst.
-      rewrite sA success_failed//=.
-      case e1: step => //[B'] vB bB0 [<-]/=.
+      rewrite sA.
+      case e1: step => //[B'] vB [<-]/=.
       move: sA; rewrite -success_cut.
       move=>/success_failed->/=.
       rewrite (HB _ _ vB e1)andbF//.
@@ -795,23 +708,18 @@ Section NurProp.
       have [sy[y[ys H]]] := failed_t2l (vA) (fA) s1 SB.
       rewrite H; case: y H => //= H [??]; subst.
       by apply: HA H.
-    - move => A HA B0 _ B HB s bt s1 xs /and3P[vA].
+    - move => A HA B0 B HB s bt s1 xs /andP[vA].
       case fA: failed => //=.
-      case: ifP => //=[sA vB bB fB|sA /eqP->{B0} bB _].
+      case: ifP => //=[sA vB fB|sA /eqP-> _ {B HB}].
         rewrite (success_t2l empty) => //=.
-        move/orPT: bB => []bB; last first.
-          rewrite base_and_ko_t2l//= make_lB01_empty2 => H.
-          by apply: HB H.
-        have [h H]:= base_and_t2l bB.
-        rewrite H/= make_lB01_empty2/=.
+        rewrite make_lB01_empty2/=.
         set ml := make_lB0 _ _.
         have [s2'[y[ys H1]]] := [elaborate failed_t2l vB (fB) (get_substS s A) (ml ++ bt)].
         rewrite H1/=.
         case: y H1 => //= H1 [??]; subst.
         by apply: HB H1.
-      have [hd H1]:= base_and_t2l bB.
-      have [s2'[y[ys H]]] := failed_t2l vA fA s bt.
-      rewrite H/=H1/=!H1/= => -[?+?]; subst.
+      have [s2'[y[ys /[dup] H ->]]]/= := failed_t2l vA fA s bt.
+      rewrite s2l_big_and => -[?+?]; subst.
       case: y H; rewrite//=cat0s => H?; subst.
       exfalso.
       apply: s2l_empty_hdF vA sA fA H.
@@ -854,17 +762,17 @@ Section NurProp.
       rewrite size_add_ca_deep size_cat -/SB ?SB'; case X: size => //[n].
       set Y:= t2l (cutr B) _ _.
       rewrite (s2l_size s1 SB) X//.
-    - move=> A HA B0 _ B HB l l1 ca tl alts s1 s2/and3P[vA].
-      case: ifP => //=[sA vB bB0|sA/eqP-> bB].
+    - move=> A HA B0 B HB l l1 ca tl alts s1 s2/andP[vA].
+      case: ifP => //=[sA vB|sA/eqP-> {B HB}].
         rewrite (success_t2l empty)//.
-        rewrite succes_is_solved//.
-        have [H|[hd[H H1]]]:= bbAnd_t2l bB0; rewrite H/=.
-          rewrite make_lB01_empty2.
+        rewrite succes_is_solved//=.
+        (* have [H|[hd[H H1]]]:= bbAnd_t2l bB0; rewrite H/=. *)
+          (* rewrite make_lB01_empty2.
           move=>/(HB _ _ _ _  _ _ _ vB).
           case e: step => //= Hz; rewrite (success_t2l empty)//=?H?success_cut//?valid_tree_cut//?size_map//.
           have vB0 := bbAnd_valid bB0.
           rewrite t2l_cutr_empty//=.
-          rewrite make_lB01_empty2 ges_subst_cutl//.
+          rewrite make_lB01_empty2 ges_subst_cutl//. *)
         set SA := t2l (odflt _ _) _ _.
         rewrite get_tree_And/=.
         case: ifP => //.
@@ -874,9 +782,8 @@ Section NurProp.
           have [hd1[tl1[Hz [Hw Hy]]]] := s2l_CutBrothers  (get_substS s1 A) (X ++ l) vB eB.
           rewrite !Hz/= => -[????]; subst.
           rewrite (success_t2l empty)?success_cut//?valid_tree_cut//=!Hw/=.
-          have vB0 := bbAnd_valid bB0.
-          by rewrite t2l_cutr_empty//=.
-        rewrite ((success_t2l empty) _ sA)//= H size_cat size_map.
+          rewrite size_cat make_lB01_empty2 size_cons//.
+        rewrite ((success_t2l empty) _ sA)//= size_cat size_map.
         set SA' := t2l (odflt _ _) _ _.
         case X : t2l => [|r rs]/=.
           rewrite cat0s.
@@ -889,30 +796,25 @@ Section NurProp.
         set Y:= make_lB0 _ _.
         have:= HB _ (Y ++ l1) _ _ _ _ _ vB X => /(_ _ IsList_alts).
         by case: t2l => //.
-      have {}bB: bbAnd B.
-        by move: bB; case:ifP => //; rewrite /bbAnd => _ ->//.
-      have [H|[hd [H Hz]]]:= bbAnd_t2l bB; rewrite H/=.
-        case: t2l => [|[]]//??; rewrite H//.
-      case SA: t2l => [|[s4 z] zs]//; rewrite H/=.
+      case SA: t2l => [|[s4 z] zs]//.
+      rewrite s2l_big_and cat_cons cat0s => -[? + ?]; subst.
       case: z SA => //=.
-        move=> Hx.
-        rewrite make_lB01_empty2.
-        move=>[??]; subst.
+        rewrite cat0s => H1 H2.
         case e: step => [A'|A'|A'|A']/=.
-        - have []:= s2l_empty_hd_success vA (step_not_failed _ e notF) Hx.
-          rewrite (step_not_solved _ e)//.
-        - have []:= s2l_empty_hd_success vA (step_not_failed _ e notF) Hx.
-          rewrite (step_not_solved _ e)//.
+        - have [] := s2l_empty_hd_success vA (step_not_failed _ e notF) H1.
+          by rewrite (step_not_solved _ e)//.
+        - have []:= s2l_empty_hd_success vA (step_not_failed _ e notF) H1.
+          by rewrite (step_not_solved _ e)//.
         - rewrite -(expand_failure_t2l_same e).
-          have {Hx} := f_equal size Hx.
+          have {H1} := f_equal size H1.
           move=>/(_ _ IsList_alts).
           rewrite (s2l_size s1 l1).
-          by case: t2l => //=[[? x] xs]; rewrite H !size_cat !size_map H//.
+          by case: t2l => //=[[? x] xs]; rewrite //=s2l_big_and//.
         - have [??]:= (expand_solved_same _ e); congruence.
-      move=> []//ca1 l2 SA []???; subst.
+      move=> []//ca1 l2 SA []??; subst.
       have:= HA _ l1 _ _ _ _ _ vA SA.
-      case e: step => [A'|A'|A'|A']/=; last first;
-        [|by (case SA': t2l => //=[[? x] xs]; rewrite H !size_cat !size_map size_add_deep H//)..].
+      case e: step => [A'|A'|A'|A']/=;
+      case: t2l => //[[s x] xs]; only 1-3: by rewrite s2l_big_and.
       have [??]:= expand_solved_same _ e; congruence.
   Qed.
 
@@ -951,16 +853,14 @@ Section NurProp.
       rewrite (expand_cb_failedF vA eA).
       move=>[????]; subst; auto.
       by rewrite (expand_cb_same_subst1 _ eA)//.
-    - move=> /= A HA B0 _ B HB s1 C s4 ca x tl l1 /and3P[vA].
+    - move=> /= A HA B0 B HB s1 C s4 ca x tl l1 /andP[vA].
       case eA: step => //[A'|A']/=.
-        rewrite (step_not_solved _ eA notF)/=(step_not_failed _ eA notF).
-        move=>/eqP->bB[<-]/=.
+        rewrite (step_not_solved _ eA notF)/=.
+        move=>/eqP->{B HB}[<-]/=.
         case SA : t2l => //[[s5 w] ws].
-        have [hd SB] := base_and_t2l bB.
-        rewrite !SB/=SB; subst.
+        rewrite s2l_big_and.
         move=>[?+?]; subst.
-        rewrite (base_and_failed bB) andbF.
-        rewrite (get_substS_base_and bB) if_same.
+        rewrite get_substS_big_and if_same.
         case: w SA => //=.
           rewrite cat0s => HH?; subst.
           exfalso.
@@ -968,7 +868,7 @@ Section NurProp.
         move=> []//=ca' gs SA []??; subst.
         have [H1 H2] := HA _ _ _ _ _ _ _ vA eA SA.
         rewrite !H1/=.
-        repeat split.
+        repeat split; first by rewrite failed_big_and andbF.
         move: H2; case SA': t2l => //=[|t ts].
           rewrite cat0s =>?; subst.
           rewrite size_cons.
@@ -978,20 +878,15 @@ Section NurProp.
           by rewrite SA'//.
         move=>[??]; subst.
         rewrite size_cat addnK drop_size_cat//add_deep_cat take_size_cat//?size_add_deep//.
-        by rewrite  SB/=.
+        by rewrite s2l_big_and.
       have [? sA]:= expand_solved_same _ eA; subst.
-      rewrite sA => /= vB bB.
+      rewrite sA => /= vB.
       case eB: step => //[B']/=[<-]//=; subst.
       rewrite (success_t2l empty vA)//=.
       rewrite sA (success_failed)//=.
-      have [H|[hd [H H3]]] := bbAnd_t2l bB; rewrite H/=.
-        rewrite !make_lB01_empty2; subst.
-        move=> H1.
-        have [H2 H3]:= HB _ _ _ _ _ _ _ vB eB H1.
-        by rewrite !H2//.
       set SA:= add_deep _ _ _.
       rewrite !make_lB01_empty2.
-      have [s[y[ys]]] := failed_t2l vB (step_not_failed _ eB notF) (get_substS s1 A') (make_lB0 SA hd ++ l1).
+      have [s[y[ys]]] := failed_t2l vB (step_not_failed _ eB notF) (get_substS s1 A') (make_lB0 SA (r2l B0.1 B0.2) ++ l1).
       move=>H4; rewrite H4/=.
       move=>[???]; subst.
       have [[H5 H5'] H6] := HB _ _ _ _ _ _ _ vB eB H4; subst.
@@ -1017,6 +912,13 @@ Section NurProp.
       rewrite save_alt_add_ca_deepA//.
     }
     case: b => //=-[pr t|[|//]] bs H; rewrite save_alt_add_ca_deepG//.
+  Qed.
+
+  Lemma empty_caG_r2l p l: empty_caG (r2l p l).
+  Proof.
+    apply: (@base_and_empty_ca (big_and p l)).
+      apply: base_and_big_and.
+    move=> ??; rewrite s2l_big_and//.
   Qed.
 
   Lemma s2l_Expanded_call {s s3 A B l p t gs xs}:
@@ -1074,16 +976,13 @@ Section NurProp.
       rewrite catA -add_ca_deep_cat.
       rewrite save_alt_add_ca_deepA//.
       apply: empty_ca_atoms1.
-    - move=> A HA B0 _ B HB C s1 s3 l p t gs xs /and3P[vA].
+    - move=> A HA B0 B HB C s1 s3 l p t gs xs /andP[vA].
       case e: step => //[A'|A'].
         have /=fA := step_not_failed _ e notF.
-        rewrite (step_not_solved _ e)//fA/=.
-        move=>/eqP->bB [<-]/=; subst.
+        rewrite (step_not_solved _ e)//.
+        move=>/eqP->{B HB} [<-]/=; subst.
         have [s5 [y[ys sA]]]:= failed_t2l vA fA s1 l.
-        have [hd H]:= base_and_t2l bB.
-        rewrite sA H/=H.
-        rewrite (base_and_failed bB) andbF orbF.
-        (* rewrite (get_substS_base_and bB). if_same. *)
+        rewrite sA/= !s2l_big_and.
         move=> [?] + ?; subst.
         case: y sA => [|[p1 t1|] tl]//=sA.
           exfalso.
@@ -1094,32 +993,31 @@ Section NurProp.
         case FF: F => [|r rs].
           move=> H1; rewrite !H1?H; split; auto.
           case: ys sA H1 => //=-[s6 y] ys sA H1.
-          by rewrite !H/make_lB01 map_cons/map/= cat_cons cat0s//.
+          by rewrite s2l_big_and /make_lB01 map_cons cat_cons cat0s//.
         move=> H1; rewrite !H1; split; auto; split => //=.
-        rewrite H/= /make_lB01 map_cons/map/= cat_cons cat0s.
+        rewrite s2l_big_and/= /make_lB01 map_cons/map/= cat_cons cat0s.
         rewrite/make_lB0 add_deep_cat map_cat.
+        set hd := (r2l B0.1 B0.2).
         rewrite-/(make_lB0 (add_deep l hd (save_alts (ys ++ l) tl (aa2gs p rs))) hd).
         rewrite-/(make_lB0 (add_deep l hd ys) hd).
-        have Hb := (base_and_empty_ca bB H).
         rewrite -!cat_cons; f_equal.
         rewrite add_deep_goalsP//?empty_ca_atoms//.
         rewrite add_deep_altsP//?empty_ca_atoms1//.
+        apply: empty_caG_r2l.
       have [? sA] := expand_solved_same _ e; subst.
-      rewrite sA success_failed//= => vB bB.
+      rewrite sA => vB.
       case e1: step => //[B'][<-]/=; subst.
       rewrite (success_failed _ sA)/=sA/=.
       rewrite (success_t2l empty)//=.
-      have [H|[hd[H H1]]]:= bbAnd_t2l bB; rewrite H/=!make_lB01_empty2.
-        by apply: HB vB e1.
       set X := make_lB0 _ _.
       set Y := get_substS _ _.
       have [s[y[ys sB]]]:= failed_t2l vB (step_not_failed _ e1 notF) Y (X++l).
-      rewrite sB cat_cons=> -[???] ; subst.
+      rewrite sB make_lB01_empty2 cat_cons => -[???] ; subst.
       have := HB _ _ _ _ _ _ _ _ vB e1 sB.
       rewrite-/Y.
       move=> []?; subst.
-      case FF: F => [|r rs].
-        by move=>Hz; subst; rewrite !Hz/=; auto.
+      case FF: F => [|r rs]; rewrite make_lB01_empty2.
+        by move=> Hz; rewrite !Hz//.
       move=>[]fB' Hz; rewrite Hz !catA//.
   Qed.
 
